theories/TypingProperties/LogRelConsequences.v
@@ -56,7 +56,7 @@ Import WeakDeclarativeTypingProperties WeakDeclarativeTypingData.
 
 End Subst.
 
-#[local, refine] Instance TypingSubstLogRel : TypingSubst (ta := de) := {}.
+#[local, refine] Instance TypingSubstLogRel : TypingSubst de := {}.
   Proof.
     all: intros ; now eapply _typing_subst.
   Qed.
@@ -119,12 +119,12 @@ Section TypeConstructors.
   Qed.
 End TypeConstructors.
 
-#[local, refine] Instance RedCompleteLogRel : TypeReductionComplete (ta := de) := {}.
+#[local, refine] Instance RedCompleteLogRel : TypeReductionComplete de := {}.
 Proof.
   all: intros ; eauto using _red_ty_complete_l, _red_ty_complete_r.
   Qed.
 
-#[local, refine] Instance TypeConstructorsInjLogRel : TypeConstructorsInj (ta := de) := {}.
+#[local, refine] Instance TypeConstructorsInjLogRel : TypeConstructorsInj de := {}.
 Proof.
   intros.
   now apply _ty_conv_inj.
@@ -331,7 +331,7 @@ Section TermConstructors.
 
 End TermConstructors.
 
-#[local, refine] Instance TermConstructorsInjLogRel : TermConstructorsInj (ta := de) := {}.
+#[local, refine] Instance TermConstructorsInjLogRel : TermConstructorsInj de := {}.
 Proof.
   - intros. now eapply _univ_conv_inj.
   - intros. now eapply _nat_conv_inj.
@@ -377,7 +377,7 @@ Section NeutralConv.
 
 End NeutralConv.
 
-#[local, refine] Instance ConvNeutralConvPosLogRel : ConvNeutralConvPos (ta := de) := {}.
+#[local, refine] Instance ConvNeutralConvPosLogRel : ConvNeutralConvPos de := {}.
 Proof.
   intros * ?? [] Hconv.
   - destruct s.
@@ -398,13 +398,13 @@ Section Completeness.
   `{!RedType ta} `{!RedTerm ta}
   `{!GenericTypingProperties ta _ _ _ _ _ _ _ _}.
 
-  #[local, refine] Instance ConvCompleteLogRel : ConvComplete (ta := de) (ta' := ta) := {}.
+  #[local, refine] Instance ConvImpliesLogRel : ConvImplies de ta := {}.
   Proof.
     - now intros * [HΓ ?%redValidTy%(escapeEq (ta := ta))]%Fundamental.
     - now intros * [HΓ ? ?%redValidTm%(escapeTm (ta := ta)) ]%Fundamental.
   Qed.
 
-  #[local, refine] Instance TypingCompleteLogRel : TypingComplete (ta := de) (ta' := ta) := {}.
+  #[local, refine] Instance TypingImpliesLogRel : TypingImplies de ta := {}.
   Proof.
     - now intros * [HΓ ?%redValidTy%(escapeTy (ta := ta))]%Fundamental.
     - now intros * [_ _ ?%redValidTm%escapeTm]%(Fundamental (ta := ta)).
@@ -561,7 +561,7 @@ Section Normalisation.
 
 End Normalisation.
 
-#[local, refine] Instance NormalisationLogRel : Normalisation (ta := de) := {}.
+#[local, refine] Instance NormalisationLogRel : Normalisation de := {}.
   Proof.
     all: intros ; eauto using _tm_norm, _ty_norm.
   Qed.
